Add interfaces to machine integer libraries

ulib/FStar.Int16.fst
@@ -1,120 +1,52 @@
 module FStar.Int16
 (* This module generated automatically using [mk_int.sh] *)
 
-let n = 16
-
 open FStar.Int
 open FStar.Mul
 
-(* NOTE: anything that you fix/update here should be reflected in [FStar.UIntN.fstp], which is mostly
- * a copy-paste of this module. *)
+(* NOTE: this file should remain synchronized with [FStar.UIntN.fstp] *)
 
 private type t' = | Mk: v:int_t n -> t'
-type t = t'
+let t = t'
 
-let v (x:t) : Tot (int_t n) = x.v
+let v x = x.v
 
-let v_inj (x1 x2: t): Lemma (requires (v x1 == v x2)) (ensures (x1 == x2)) = ()
+let v_inj x1 x2 = ()
 
-val add: a:t -> b:t -> Pure t
-  (requires (size (v a + v b) n))
-  (ensures (fun c -> v a + v b = v c))
-let add a b =
-  Mk (add (v a) (v b))
+let add a b = Mk (add (v a) (v b))
 
 (* Subtraction primitives *)
-val sub: a:t -> b:t -> Pure t
-  (requires (size (v a - v b) n))
-  (ensures (fun c -> v a - v b = v c))
-let sub a b =
-  Mk (sub (v a) (v b))
+let sub a b = Mk (sub (v a) (v b))
 
 (* Multiplication primitives *)
-val mul: a:t -> b:t -> Pure t
-  (requires (size (v a * v b) n))
-  (ensures (fun c -> v a * v b = v c))
-let mul a b =
-  Mk (mul (v a) (v b))
+let mul a b = Mk (mul (v a) (v b))
 
 (* Division primitives *)
-val div: a:t -> b:t{v b <> 0} -> Pure t
-  // division overflows on INT_MIN / -1
-  (requires (size (v a / v b) n))
-  (ensures (fun c -> v a / v b = v c))
-let div a b =
-  Mk (div (v a) (v b))
+let div a b = Mk (div (v a) (v b))
 
 (* Modulo primitives *)
-val rem: a:t -> b:t{v b <> 0} -> Pure t
-  (requires True)
-  (ensures (fun c ->
-    v a - ((v a / v b) * v b) = v c))
 let rem a b = Mk (mod (v a) (v b))
 
 (* Bitwise operators *)
-val logand: t -> t -> Tot t
 let logand a b = Mk (logand (v a) (v b))
-val logxor: t -> t -> Tot t
 let logxor a b = Mk (logxor (v a) (v b))
-val logor: t -> t -> Tot t
 let logor a b = Mk (logor (v a) (v b))
-val lognot: t -> Tot t
 let lognot a = Mk (lognot (v a))
 
-val int_to_t: x:int_t n -> Pure t
-  (requires True)
-  (ensures (fun y -> v y = x))
 let int_to_t x = Mk x
 
-#set-options "--lax"
-//This private primitive is used internally by the
-//compiler to translate bounded integer constants
-//with a desugaring-time check of the size of the number,
-//rather than an expensive verifiation check.
-//Since it is marked private, client programs cannot call it directly
-//Since it is marked unfold, it eagerly reduces,
-//eliminating the verification overhead of the wrapper
-private
-unfold
-let __int_to_t (x:int) : Tot t
-    = int_to_t x
-#reset-options
-
 (* Shift operators *)
-val shift_right: a:t -> s:UInt32.t -> Pure t
-  (requires (UInt32.v s < n))
-  (ensures (fun c -> v c = (v a /% (pow2 (UInt32.v s)))))
 let shift_right a s = Mk (shift_right (v a) (UInt32.v s))
 
-val shift_left: a:t -> s:UInt32.t -> Pure t
-  (requires (UInt32.v s < n))
-  (ensures (fun c -> v c = ((v a * pow2 (UInt32.v s)) @% pow2 n)))
 let shift_left a s = Mk (shift_left (v a) (UInt32.v s))
 
 (* Comparison operators *)
-let eq (a:t) (b:t) : Tot bool = eq #n (v a) (v b)
-let gt (a:t) (b:t) : Tot bool = gt #n (v a) (v b)
-let gte (a:t) (b:t) : Tot bool = gte #n (v a) (v b)
-let lt (a:t) (b:t) : Tot bool = lt #n (v a) (v b)
-let lte (a:t) (b:t) : Tot bool = lte #n (v a) (v b)
-
-(* Infix notations *)
-unfold let op_Plus_Hat = add
-unfold let op_Subtraction_Hat = sub
-unfold let op_Star_Hat = mul
-unfold let op_Slash_Hat = div
-unfold let op_Percent_Hat = rem
-unfold let op_Hat_Hat = logxor
-unfold let op_Amp_Hat = logand
-unfold let op_Bar_Hat = logor
-unfold let op_Less_Less_Hat = shift_left
-unfold let op_Greater_Greater_Hat = shift_right
-unfold let op_Equals_Hat = eq
-unfold let op_Greater_Hat = gt
-unfold let op_Greater_Equals_Hat = gte
-unfold let op_Less_Hat = lt
-unfold let op_Less_Equals_Hat = lte
+let eq a b = eq #n (v a) (v b)
+let gt a b = gt #n (v a) (v b)
+let gte a b = gte #n (v a) (v b)
+let lt a b = lt #n (v a) (v b)
+let lte a b = lte #n (v a) (v b)
 
 (* To input / output constants *)
-assume val to_string: t -> Tot string
-assume val of_string: string -> Tot t
+let to_string = admit()
+let of_string = admit()
