ulib/FStar.UInt16.fst
@@ -1,180 +1,69 @@
 module FStar.UInt16
 (* This module generated automatically using [mk_int.sh] *)
 
-let n = 16
-
 open FStar.UInt
 open FStar.Mul
 
-(* NOTE: anything that you fix/update here should be reflected in [FStar.IntN.fstp], which is mostly
- * a copy-paste of this module. *)
-
-(* This is really the same thing as [FStar.IntN.fstp], with:
- * - every occurrence of [int_t] has been replaced with [uint_t]
- * - every occurrence of [@%] has been replaced with [%].
- *)
+(* NOTE: this file should remain synchronized with [FStar.IntN.fstp] *)
 
 private type t' = | Mk: v:uint_t n -> t'
-type t = t'
+let t = t'
 
-let v (x:t) : Tot (uint_t n) = x.v
+let v x = x.v
 
-let v_inj (x1 x2: t): Lemma (requires (v x1 == v x2)) (ensures (x1 == x2)) = ()
+let v_inj x1 x2 = ()
 
-val add: a:t -> b:t -> Pure t
-  (requires (size (v a + v b) n))
-  (ensures (fun c -> v a + v b = v c))
-let add a b =
-  Mk (add (v a) (v b))
+let add a b = Mk (add (v a) (v b))
 
-val add_underspec: a:t -> b:t -> Pure t
-  (requires True)
-  (ensures (fun c ->
-    size (v a + v b) n ==> v a + v b = v c))
-let add_underspec a b =
-  Mk (add_underspec (v a) (v b))
+let add_underspec a b = Mk (add_underspec (v a) (v b))
 
-val add_mod: a:t -> b:t -> Pure t
-  (requires True)
-  (ensures (fun c -> (v a + v b) % pow2 n = v c))
-let add_mod a b =
-  Mk (add_mod (v a) (v b))
+let add_mod a b = Mk (add_mod (v a) (v b))
 
 (* Subtraction primitives *)
-val sub: a:t -> b:t -> Pure t
-  (requires (size (v a - v b) n))
-  (ensures (fun c -> v a - v b = v c))
-let sub a b =
-  Mk (sub (v a) (v b))
+let sub a b = Mk (sub (v a) (v b))
 
-val sub_underspec: a:t -> b:t -> Pure t
-  (requires True)
-  (ensures (fun c ->
-    size (v a - v b) n ==> v a - v b = v c))
-let sub_underspec a b =
-  Mk (sub_underspec (v a) (v b))
+let sub_underspec a b = Mk (sub_underspec (v a) (v b))
 
-val sub_mod: a:t -> b:t -> Pure t
-  (requires True)
-  (ensures (fun c -> (v a - v b) % pow2 n = v c))
-let sub_mod a b =
-  Mk (sub_mod (v a) (v b))
+let sub_mod a b = Mk (sub_mod (v a) (v b))
 
 (* Multiplication primitives *)
-val mul: a:t -> b:t -> Pure t
-  (requires (size (v a * v b) n))
-  (ensures (fun c -> v a * v b = v c))
-let mul a b =
-  Mk (mul (v a) (v b))
+let mul a b = Mk (mul (v a) (v b))
 
-val mul_underspec: a:t -> b:t -> Pure t
-  (requires True)
-  (ensures (fun c ->
-    size (v a * v b) n ==> v a * v b = v c))
-let mul_underspec a b =
-  Mk (mul_underspec (v a) (v b))
+let mul_underspec a b = Mk (mul_underspec (v a) (v b))
 
-val mul_mod: a:t -> b:t -> Pure t
-  (requires True)
-  (ensures (fun c -> (v a * v b) % pow2 n = v c))
-let mul_mod a b =
-  Mk (mul_mod (v a) (v b))
+let mul_mod a b = Mk (mul_mod (v a) (v b))
 
-val mul_div: a:t -> b:t -> Pure t
-  (requires True)
-  (ensures (fun c -> (v a * v b) / pow2 n = v c))
-let mul_div a b =
-  Mk (mul_div (v a) (v b))
+let mul_div a b = Mk (mul_div (v a) (v b))
 
 (* Division primitives *)
-val div: a:t -> b:t{v b <> 0} -> Pure t
-  (requires (True))
-  (ensures (fun c -> v a / v b = v c))
-let div a b =
-  Mk (div (v a) (v b))
+let div a b = Mk (div (v a) (v b))
 
 (* Modulo primitives *)
-val rem: a:t -> b:t{v b <> 0} -> Pure t
-  (requires True)
-  (ensures (fun c ->
-    v a - ((v a / v b) * v b) = v c))
 let rem a b = Mk (mod (v a) (v b))
 
 (* Bitwise operators *)
-val logand: t -> t -> Tot t
 let logand a b = Mk (logand (v a) (v b))
-val logxor: t -> t -> Tot t
 let logxor a b = Mk (logxor (v a) (v b))
-val logor: t -> t -> Tot t
 let logor a b = Mk (logor (v a) (v b))
-val lognot: t -> Tot t
 let lognot a = Mk (lognot (v a))
 
-val uint_to_t: x:uint_t n -> Pure t
-  (requires True)
-  (ensures (fun y -> v y = x))
 let uint_to_t x = Mk x
 
-#set-options "--lax"
-//This private primitive is used internally by the
-//compiler to translate bounded integer constants
-//with a desugaring-time check of the size of the number,
-//rather than an expensive verifiation check.
-//Since it is marked private, client programs cannot call it directly
-//Since it is marked unfold, it eagerly reduces,
-//eliminating the verification overhead of the wrapper
-private
-unfold
-let __uint_to_t (x:int) : Tot t
-    = uint_to_t x
-#reset-options
-
-
 (* Shift operators *)
-val shift_right: a:t -> s:UInt32.t -> Pure t
-  (requires (UInt32.v s < n))
-  (ensures (fun c -> v c = (v a / (pow2 (UInt32.v s)))))
-let shift_right a s = Mk (shift_right (v a) (UInt32.v s))
+let shift_right a s = Mk (shift_right (v a) (v s))
 
-val shift_left: a:t -> s:UInt32.t -> Pure t
-  (requires (UInt32.v s < n))
-  (ensures (fun c -> v c = ((v a * pow2 (UInt32.v s)) % pow2 n)))
-let shift_left a s = Mk (shift_left (v a) (UInt32.v s))
+let shift_left a s = Mk (shift_left (v a) (v s))
 
 (* Comparison operators *)
-let eq (a:t) (b:t) : Tot bool = eq #n (v a) (v b)
-let gt (a:t) (b:t) : Tot bool = gt #n (v a) (v b)
-let gte (a:t) (b:t) : Tot bool = gte #n (v a) (v b)
-let lt (a:t) (b:t) : Tot bool = lt #n (v a) (v b)
-let lte (a:t) (b:t) : Tot bool = lte #n (v a) (v b)
+let eq a b = eq #n (v a) (v b)
+let gt a b = gt #n (v a) (v b)
+let gte a b = gte #n (v a) (v b)
+let lt a b = lt #n (v a) (v b)
+let lte a b = lte #n (v a) (v b)
 
-assume val eq_mask: a:t -> b:t -> Tot (c:t{(v a = v b ==> v c = pow2 n - 1) /\ (v a <> v b ==> v c = 0)})
-assume val gte_mask: a:t -> b:t -> Tot (c:t{(v a >= v b ==> v c = pow2 n - 1) /\ (v a < v b ==> v c = 0)})
-
-(* Infix notations *)
-unfold let op_Plus_Hat = add
-unfold let op_Plus_Question_Hat = add_underspec
-unfold let op_Plus_Percent_Hat = add_mod
-unfold let op_Subtraction_Hat = sub
-unfold let op_Subtraction_Question_Hat = sub_underspec
-unfold let op_Subtraction_Percent_Hat = sub_mod
-unfold let op_Star_Hat = mul
-unfold let op_Star_Question_Hat = mul_underspec
-unfold let op_Star_Percent_Hat = mul_mod
-unfold let op_Star_Slash_Hat = mul_div
-unfold let op_Slash_Hat = div
-unfold let op_Percent_Hat = rem
-unfold let op_Hat_Hat = logxor
-unfold let op_Amp_Hat = logand
-unfold let op_Bar_Hat = logor
-unfold let op_Less_Less_Hat = shift_left
-unfold let op_Greater_Greater_Hat = shift_right
-unfold let op_Equals_Hat = eq
-unfold let op_Greater_Hat = gt
-unfold let op_Greater_Equals_Hat = gte
-unfold let op_Less_Hat = lt
-unfold let op_Less_Equals_Hat = lte
+let eq_mask a b = if eq a b then Mk (pow2 n - 1) else Mk 0
+let gte_mask a b = if gte a b then Mk (pow2 n - 1) else Mk 0
 
 (* To input / output constants *)
-assume val to_string: t -> Tot string
-assume val of_string: string -> Tot t
+let to_string = admit()
+let of_string = admit()
