ulib/FStar.Int64.fsti
@@ -1,0 +1,127 @@
+module FStar.Int64
+(* This module generated automatically using [mk_int.sh] *)
+
+let n = 64
+
+open FStar.Int
+open FStar.Mul
+
+(* NOTE: this file should remain synchronized with [FStar.UIntN.fstip] *)
+
+(* This is really the same thing as [FStar.UIntN.fstp], with:
+  * - every occurrence of [uint_t] has been replaced with [int_t]
+  * - every occurrence of [%] has been replaced with [@%].
+  * - every occurrence of [/] has been replaced with [/%].
+  * - the *_mod and *_underspec arithmetic functions have been removed since
+      they have undefined behavior in C
+  *)
+
+val t: t:Type0{hasEq t}
+
+val v : t -> int_t n
+
+val v_inj : x1:t -> x2:t ->
+  Lemma (requires (v x1 == v x2))
+        (ensures (x1 == x2))
+
+val add: a:t -> b:t -> Pure t
+  (requires (size (v a + v b) n))
+  (ensures (fun c -> v a + v b = v c))
+
+(* Subtraction primitives *)
+val sub: a:t -> b:t -> Pure t
+  (requires (size (v a - v b) n))
+  (ensures (fun c -> v a - v b = v c))
+
+(* Multiplication primitives *)
+val mul: a:t -> b:t -> Pure t
+  (requires (size (v a * v b) n))
+  (ensures (fun c -> v a * v b = v c))
+
+(* Division primitives *)
+val div: a:t -> b:t{v b <> 0} -> Pure t
+  (requires (size (v a / v b) n))
+  (ensures (fun c -> v a / v b = v c))
+
+(* Modulo primitives *)
+val rem: a:t -> b:t{v b <> 0} -> Pure t
+  (requires True)
+  (ensures (fun c ->
+    v a - ((v a / v b) * v b) = v c))
+
+(* Bitwise operators *)
+val logand: a:t -> b:t -> Pure t
+  (requires True)
+  (ensures (fun r -> v r = logand (v a) (v b)))
+val logxor: a:t -> b:t -> Pure t
+  (requires True)
+  (ensures (fun r -> v r = logxor (v a) (v b)))
+val logor: a:t -> b:t -> Pure t
+  (requires True)
+  (ensures (fun r -> v r = logor (v a) (v b)))
+val lognot: a:t -> Pure t
+  (requires True)
+  (ensures (fun r -> v r = lognot (v a)))
+
+val int_to_t: x:int_t n -> Pure t
+  (requires True)
+  (ensures (fun y -> v y = x))
+
+//This private primitive is used internally by the
+//compiler to translate bounded integer constants
+//with a desugaring-time check of the size of the number,
+//rather than an expensive verification check.
+//Since it is marked private, client programs cannot call it directly
+//Since it is marked unfold, it eagerly reduces,
+//eliminating the verification overhead of the wrapper
+private
+unfold
+let __int_to_t (x:int) : Tot t
+    = admit(); int_to_t x
+
+(* Shift operators *)
+val shift_right: a:t -> s:UInt32.t -> Pure t
+  (requires (UInt32.v s < n))
+  (ensures (fun c -> v c = (v a /% (pow2 (UInt32.v s)))))
+
+val shift_left: a:t -> s:UInt32.t -> Pure t
+  (requires (UInt32.v s < n))
+  (ensures (fun c -> v c = ((v a * pow2 (UInt32.v s)) @% pow2 n)))
+
+(* Comparison operators *)
+val eq : a:t -> b:t -> Pure bool
+  (requires True)
+  (ensures (fun r -> r == (v a = v b)))
+val gt : a:t -> b:t -> Pure bool
+  (requires True)
+  (ensures (fun r -> r == (v a > v b)))
+val gte : a:t -> b:t -> Pure bool
+  (requires True)
+  (ensures (fun r -> r == (v a >= v b)))
+val lt : a:t -> b:t -> Pure bool
+  (requires True)
+  (ensures (fun r -> r == (v a < v b)))
+val lte : a:t -> b:t -> Pure bool
+  (requires True)
+  (ensures (fun r -> r == (v a <= v b)))
+
+(* Infix notations *)
+unfold let op_Plus_Hat = add
+unfold let op_Subtraction_Hat = sub
+unfold let op_Star_Hat = mul
+unfold let op_Slash_Hat = div
+unfold let op_Percent_Hat = rem
+unfold let op_Hat_Hat = logxor
+unfold let op_Amp_Hat = logand
+unfold let op_Bar_Hat = logor
+unfold let op_Less_Less_Hat = shift_left
+unfold let op_Greater_Greater_Hat = shift_right
+unfold let op_Equals_Hat = eq
+unfold let op_Greater_Hat = gt
+unfold let op_Greater_Equals_Hat = gte
+unfold let op_Less_Hat = lt
+unfold let op_Less_Equals_Hat = lte
+
+(* To input / output constants *)
+val to_string: t -> Tot string
+val of_string: string -> Tot t
