ulib/mk_int.sh
@@ -1,7 +1,8 @@
 #!/usr/bin/env bash
 
 for i in 8 16 31 32 63 64 128; do
-  f=FStar.Int$i.fst
+  # generate interface
+  f=FStar.Int$i.fsti
   cat > $f <<EOF
 module FStar.Int$i
 (* This module generated automatically using [mk_int.sh] *)
@@ -9,14 +10,28 @@ module FStar.Int$i
 let n = $i
 
 EOF
-  cat FStar.IntN.fstp >> $f
+  cat FStar.IntN.fstip >> $f
   if [ $i -eq 128 ]; then
       cat >> $f <<EOF
 
 val mul_wide: a:Int64.t -> b:Int64.t -> Pure t
   (requires True)
   (ensures (fun c -> v c = Int64.v a * Int64.v b))
-let mul_wide a b = 
+EOF
+  fi
+
+  # generate implementation
+  f=FStar.Int$i.fst
+  cat > $f <<EOF
+module FStar.Int$i
+(* This module generated automatically using [mk_int.sh] *)
+
+EOF
+  cat FStar.IntN.fstp >> $f
+  if [ $i -eq 128 ]; then
+      cat >> $f <<EOF
+
+let mul_wide a b =
   assume (size (Int64.v a * Int64.v b) n);
   Mk ((Int64.v a) * (Int64.v b))
 EOF
@@ -24,7 +39,8 @@ EOF
 done
 
 for i in 8 16 31 32 63 64; do
-  f=FStar.UInt$i.fst
+  # generate interface
+  f=FStar.UInt$i.fsti
   cat > $f <<EOF
 module FStar.UInt$i
 (* This module generated automatically using [mk_int.sh] *)
@@ -32,21 +48,28 @@ module FStar.UInt$i
 let n = $i
 
 EOF
+  cat FStar.UIntN.fstip >> $f
+  if [ $i -eq 8 ]; then
+      cat >> $f <<EOF
+unfold inline_for_extraction let byte = t
+// workaround for issue #1088
+val __dummy: unit
+EOF
+  fi
+
+  # generate implementation
+  f=FStar.UInt$i.fst
+  cat > $f <<EOF
+module FStar.UInt$i
+(* This module generated automatically using [mk_int.sh] *)
+
+EOF
   cat FStar.UIntN.fstp >> $f
   if [ $i -eq 8 ]; then
-    echo "unfold inline_for_extraction type byte = t" >> $f
-  fi
-  if [ $i -eq 128 ]; then
       cat >> $f <<EOF
-
-val mul_wide: a:UInt64.t -> b:UInt64.t -> Pure t
-  (requires True)
-  (ensures (fun c -> v c = UInt64.v a * UInt64.v b))
-let mul_wide a b = 
-  assume (size (UInt64.v a * UInt64.v b) n);
-  Mk ((UInt64.v a) * (UInt64.v b))
+let __dummy = ()
 EOF
   fi
 done
 
-sed -i.bak 's/UInt32.//g' FStar.UInt32.fst
+sed -i.bak 's/UInt32\.//g' FStar.UInt32.fst
